

Effective length of column

Length of column

$$l_c := 6 \text{ } m$$

$$\mu_i(U, R) := \begin{cases} \text{if } U_0 = \text{"fixed"} \wedge R_0 = \text{"free"} \wedge (U_1 = \text{"fixed"} \wedge R_1 = \text{"free"}) \\ \parallel 1 \\ \text{else if } U_0 = \text{"free"} \wedge R_0 = \text{"free"} \wedge (U_1 = \text{"fixed"} \wedge R_1 = \text{"fixed"}) \\ \parallel 2 \\ \text{else if } U_0 = \text{"fixed"} \wedge R_0 = \text{"fixed"} \wedge (U_1 = \text{"free"} \wedge R_1 = \text{"free"}) \\ \parallel 2 \\ \text{else if } U_0 = \text{"fixed"} \wedge R_0 = \text{"free"} \wedge (U_1 = \text{"fixed"} \wedge R_1 = \text{"fixed"}) \\ \parallel 0.7 \\ \text{else if } U_0 = \text{"fixed"} \wedge R_0 = \text{"fixed"} \wedge (U_1 = \text{"fixed"} \wedge R_1 = \text{"free"}) \\ \parallel 0.7 \\ \text{else if } U_0 = \text{"fixed"} \wedge R_0 = \text{"free"} \wedge (U_1 = \text{"fixed"} \wedge R_1 = \text{"lim"}) \\ \parallel 0.9 \\ \text{else if } U_0 = \text{"fixed"} \wedge R_0 = \text{"lim"} \wedge (U_1 = \text{"fixed"} \wedge R_1 = \text{"free"}) \\ \parallel 0.9 \\ \text{else if } U_0 = \text{"lim"} \wedge R_0 = \text{"free"} \wedge (U_1 = \text{"fixed"} \wedge R_1 = \text{"fixed"}) \\ \parallel 1.5 \\ \text{else if } U_0 = \text{"fixed"} \wedge R_0 = \text{"fixed"} \wedge (U_1 = \text{"lim"} \wedge R_1 = \text{"free"}) \\ \parallel 1.5 \\ \text{else if } U_0 = \text{"lim"} \wedge R_0 = \text{"free"} \wedge (U_1 = \text{"lim"} \wedge R_1 = \text{"fixed"}) \\ \parallel 2 \\ \text{else if } U_0 = \text{"lim"} \wedge R_0 = \text{"fixed"} \wedge (U_1 = \text{"lim"} \wedge R_1 = \text{"free"}) \\ \parallel 2 \\ \text{else if } U_0 = \text{"fixed"} \wedge R_0 = \text{"fixed"} \wedge (U_1 = \text{"fixed"} \wedge R_1 = \text{"fixed"}) \\ \parallel 0.5 \\ \text{else if } U_0 = \text{"fixed"} \wedge R_0 = \text{"lim"} \wedge (U_1 = \text{"fixed"} \wedge R_1 = \text{"lim"}) \\ \parallel 0.8 \\ \text{else if } U_0 = \text{"lim"} \wedge R_0 = \text{"fixed"} \wedge (U_1 = \text{"lim"} \wedge R_1 = \text{"fixed"}) \\ \parallel 0.8 \\ \text{else if } U_0 = \text{"lim"} \wedge R_0 = \text{"lim"} \wedge (U_1 = \text{"lim"} \wedge R_1 = \text{"lim"}) \\ \parallel 1.2 \\ \text{else} \\ \parallel \text{"undefined"} \end{cases}$$

$Point_x$ U_{ix} R_{ix}

“Top” “fixed” “free”
“Bottom” “fixed” “fixed”

$$\mu_x := \mu_i(U_{ix}, R_{ix}) = 0.7$$

$$st_x := \left\| \begin{array}{l} \text{if } U_{ix_0} = \text{“fixed”} \wedge R_{ix_0} = \text{“free”} \wedge (U_{ix_1} = \text{“fixed”} \wedge R_{ix_1} = \text{“free”}) \\ \quad \left\| s \leftarrow \text{“def”} \right. \\ \text{else if } U_{ix_0} = \text{“free”} \wedge R_{ix_0} = \text{“free”} \wedge (U_{ix_1} = \text{“fixed”} \wedge R_{ix_1} = \text{“fixed”}) \\ \quad \left\| s \leftarrow \text{“def”} \right. \\ \text{else if } U_{ix_0} = \text{“fixed”} \wedge R_{ix_0} = \text{“fixed”} \wedge (U_{ix_1} = \text{“free”} \wedge R_{ix_1} = \text{“free”}) \\ \quad \left\| s \leftarrow \text{“def”} \right. \\ \text{else} \\ \quad \left\| s \leftarrow \text{“indef”} \right. \\ s \end{array} \right\| = \text{“indef”}$$

$Point_y$ U_{iy} R_{iy}

“Top” “fixed” “free”
“Bottom” “fixed” “fixed”

$$\mu_y := \mu_i(U_{iy}, R_{iy}) = 0.7$$

$$st_y := \left\| \begin{array}{l} \text{if } U_{iy_0} = \text{“fixed”} \wedge R_{iy_0} = \text{“free”} \wedge (U_{iy_1} = \text{“fixed”} \wedge R_{iy_1} = \text{“free”}) \\ \quad \left\| s \leftarrow \text{“def”} \right. \\ \text{else if } U_{iy_0} = \text{“free”} \wedge R_{iy_0} = \text{“free”} \wedge (U_{iy_1} = \text{“fixed”} \wedge R_{iy_1} = \text{“fixed”}) \\ \quad \left\| s \leftarrow \text{“def”} \right. \\ \text{else if } U_{iy_0} = \text{“fixed”} \wedge R_{iy_0} = \text{“fixed”} \wedge (U_{iy_1} = \text{“free”} \wedge R_{iy_1} = \text{“free”}) \\ \quad \left\| s \leftarrow \text{“def”} \right. \\ \text{else} \\ \quad \left\| s \leftarrow \text{“indef”} \right. \\ s \end{array} \right\| = \text{“indef”}$$